Finished formalizing 9.2 and began exercises

jkstpierre/Unification.v
@@ -6,6 +6,12 @@
 
 Require Import List.
 Require Import Basics.
+Require Import Logic.
+Require Import Arith.EqNat.
+Require Import Nat.
+Import ListNotations.
+
+(* Begin 9.1 Definitions *)
 
 Definition var := nat.
 
@@ -44,63 +50,157 @@ Lemma subst_term_var_agreement :
         forall s, (sigma s) = (tau s).
 Proof.
   intros sigma tau sub1 sub2 var_agree s. induction s.
-  - apply var_agree.
-  - unfold subst in sub1. unfold subst in sub2. rewrite sub1. 
-  rewrite sub2. rewrite IHs1. rewrite IHs2. reflexivity.
+    - apply var_agree.
+    - unfold subst in sub1. unfold subst in sub2. rewrite sub1. rewrite sub2. rewrite IHs1. rewrite IHs2. reflexivity.
 Qed.
 
 (* Exercise 9.1.2 *)
 Lemma principle_unif_idempotent :
-forall sigma A, principal_unifier sigma A -> (forall t, (sigma (sigma t)) = (sigma t)).
+  forall sigma A, principal_unifier sigma A -> (forall t, (sigma (sigma t)) = (sigma t)).
 Proof.
-intros. unfold principal_unifier in H. destruct H. apply H0. apply H.
+  intros. unfold principal_unifier in H. destruct H. apply H0. apply H.
 Qed.
 
 (* Exercise 9.1.3 part A *)
 Lemma unif_fact_a :
-forall A t s sigma, unif sigma ((s, t) :: A) <-> (sigma s) = (sigma t) /\ unif sigma A.
+  forall A t s sigma, unif sigma ((s, t) :: A) <-> (sigma s) = (sigma t) /\ unif sigma A.
 Proof.
-intros. split.
-- intros. firstorder.
-- intros. firstorder. inversion H2. symmetry in H4. symmetry in H5. rewrite H4. rewrite H5. apply H.
+  intros. split.
+    - intros. firstorder.
+    - intros. firstorder. inversion H2. symmetry in H4. symmetry in H5. rewrite H4. rewrite H5. apply H.
 Qed.
 
 (* Exercise 9.1.3 part B *)
 Lemma unif_fact_b :
-forall A B sigma, unif sigma (A ++ B) <-> (unif sigma A) /\ (unif sigma B).
+  forall A B sigma, unif sigma (A ++ B) <-> (unif sigma A) /\ (unif sigma B).
 Proof.
-intros. split. 
-- intros. split.
-+ induction B.
-* rewrite app_nil_r in H. apply H.
-* apply IHB. unfold unif in H. destruct H. unfold unif. split. apply H. intros. apply H0. apply in_app_or in H1. apply in_app_iff with (l':= a :: B).
-destruct H1.
-{ left. apply H1. }
-{ right. apply in_cons. apply H1. }
-+ induction A.
-* simpl in H. apply H.
-* apply IHA. unfold unif in H. destruct H. unfold unif. split. apply H. intros. apply H0. apply in_app_or in H1. apply in_app_iff with (l := a :: A). 
-destruct H1.
-{ left. apply in_cons. apply H1. }
-{ right. apply H1. }
-- intros. unfold unif in *. destruct H. destruct H. destruct H0. split. apply H. intros. 
-apply in_app_or in H3. destruct H3.
-{ apply H1. apply H3. }
-{ apply H2. apply H3. }
+  intros. split. 
+    - intros. split.
+      + induction B.
+        * rewrite app_nil_r in H. apply H.
+        * apply IHB. unfold unif in H. destruct H. unfold unif. split. apply H. intros. apply H0. apply in_app_or in H1. apply in_app_iff with (l':= a :: B). destruct H1.
+          { left. apply H1. }
+          { right. apply in_cons. apply H1. }
+      + induction A.
+        * simpl in H. apply H.
+        * apply IHA. unfold unif in H. destruct H. unfold unif. split. apply H. intros. apply H0. apply in_app_or in H1. apply in_app_iff with (l := a :: A). destruct H1.
+          { left. apply in_cons. apply H1. }
+          { right. apply H1. }
+    - intros. unfold unif in *. destruct H. destruct H. destruct H0. split. apply H. intros. apply in_app_or in H3. destruct H3.
+      + apply H1. apply H3.
+      + apply H2. apply H3. 
 Qed.
 
 (* Exercise 9.1.4 *)
 Lemma sublist_non_unifiable :
-forall A B, incl A B -> (unifiable B) -> (unifiable A).
+  forall A B, incl A B -> (unifiable B) -> (unifiable A).
 Proof.
-intros. unfold unifiable in *. firstorder.
+  intros. unfold unifiable in *. firstorder.
 Qed.
 
+(* Begin 9.2 Definitions *)
 
+Fixpoint v_term t :=
+match t with 
+  | (V x) => [x]
+  | (T s t) => (v_term s) ++ (v_term t)
+end.
 
+Fixpoint v_list A :=
+match A with
+  | nil => nil
+  | st :: A' => (v_term (fst st)) ++ (v_term (snd st)) ++ (v_list A')
+end.
 
+Fixpoint domain A :=
+match A with
+  | nil => nil
+  | (V x, _) :: A' => x :: (domain A')
+  | _ :: A' => nil
+end.
 
+Definition disjoint {X} (A B : list X) : Prop :=
+  ~ (exists x:X, In x A /\ In x B).
 
+Inductive solved : list eqn -> Prop :=
+  | solved_nil : solved nil
+  | solved_cons : forall x s A, ~(In x (v_term s)) -> ~(In x (domain A)) -> (disjoint (v_term s) (domain A)) -> (solved A) -> (solved ((V x, s) :: A)).
 
+Fixpoint var_term_replace s x t :=
+match s with
+  | (V y) => 
+    if (beq_nat x y) 
+      then t 
+    else (V y)
+  | (T u v) => (T (var_term_replace u x t) (var_term_replace v x t))
+end.
 
+Fixpoint var_list_replace A x t :=
+match A with
+  | nil => nil
+  | uv :: A' => ((var_term_replace (fst uv) x t), (var_term_replace (snd uv) x t)) :: (var_list_replace A' x t)
+end.
 
+Fixpoint phi A s :=
+match A with
+  | nil => s
+  | (V x, t) :: A' => var_term_replace (phi A' s) x t
+  | (u, v) :: A' => s
+end.
+
+Lemma solved_principle_unifier :
+  forall A, (solved A) -> (principal_unifier (phi A) A).
+Proof.
+  intros.
+Admitted.
+
+(* 9.2.3 Part A *)
+Fact var_term_no_replacement :
+  forall x s t,
+    ~ (In x (v_term s)) -> (var_term_replace s x t) = s.
+Proof.
+  intros. unfold not in H. induction s.
+    - simpl. simpl in H. firstorder. destruct (beq_nat x v) eqn:H0.
+      + apply beq_nat_true in H0. exfalso. apply H. symmetry in H0. apply H0.
+      + reflexivity.
+    - simpl in *. apply f_equal2. 
+      + firstorder.
+      + firstorder.
+Qed.
+
+(* 9.2.3 Part B *)
+Fact var_list_no_replacement :
+  forall x A t,
+    ~ (In x (v_list A)) -> (var_list_replace A x t) = A.
+Proof.
+  intros. unfold not in H. induction A.
+    - simpl. reflexivity.
+    - simpl. apply f_equal2.
+      + destruct a. simpl. apply f_equal2.
+        * simpl in H. apply var_term_no_replacement. intros H0. apply H. apply in_or_app. left. apply H0.
+        * simpl in H. apply var_term_no_replacement. intros H0. apply H. apply in_or_app. right. apply in_or_app. left. apply H0.
+      + apply IHA. firstorder. apply H. apply in_or_app. right. apply in_or_app. right. apply H0.
+Qed.
+
+(* 9.2.3 Part C *)
+Fact term_list_domain_agreement : 
+  forall x A t,
+    ~ (In x (domain A)) -> (domain (var_list_replace A x t)) = (domain A).
+Proof.
+  intros. unfold not in H. induction A.
+    - simpl. reflexivity.
+    - destruct a. destruct t0.
+      + destruct (beq_nat x v) eqn:H0.
+        * exfalso. apply H. simpl. left. apply beq_nat_true in H0. symmetry in H0. apply H0.
+        * simpl. rewrite H0. apply f_equal2.
+          { reflexivity. }
+          { apply IHA. intros. apply H. simpl. right. apply H1. }
+      + firstorder.
+Qed.
+
+(* 9.2.3 Part D *)
+Fact subst_replacement :
+  forall sigma s x t,
+    (subst sigma) -> (sigma (V x)) = (sigma t) -> (sigma (var_term_replace s x t)) = (sigma s).
+Proof.
+  intros. induction s.
